

$$\int u dv = uv - \int v du.$$

• 1214.  $\int \ln x dx.$

• 1215.  $\int xe^{2x} dx.$

1216.  $\int \operatorname{arctg} x dx.$

• 1217.  $\int x \cos x dx.$

1218.  $\int x \operatorname{arctg} x dx.$

1219.  $\int \frac{x}{\sin^2 x} dx.$

1220.  $\int \frac{\ln x}{x^2} dx.$

1221.  $\int \sqrt{x} \ln x dx.$

1222.  $\int x^n \ln x dx.$

1223.  $\int \frac{x \cos x}{\sin^3 x} dx.$

1224.  $\int \arcsin x dx.$

$\checkmark \ln f(x)$        $\checkmark P_n(x) \cdot a^x$        $\checkmark a^x \cdot \sin x$   
 $\checkmark \arccos f(x)$        $\checkmark P_n(x) \cdot \sin x$

$$\frac{A}{(x^2+a^2)^n}$$

$$\int \underbrace{\ln x}_u \underbrace{dx}_{dv} = \left. \begin{array}{l} \ln x = u \quad du = d \ln x = \frac{1}{x} \cdot dx \\ dx = dv \quad v = x \end{array} \right| = \ln x \cdot x - \int x \cdot \frac{1}{x} dx -$$

$$= x \ln x - \int dx = x \ln x - x +$$

$$\int \underbrace{x}_u \cdot \underbrace{e^{2x}}_{dv} dx = \left| \begin{array}{l} u=x \quad du=dx \\ e^{2x} dx = dv \quad v = \frac{1}{2} e^{2x} \end{array} \right| = x \cdot \frac{1}{2} e^{2x} - \frac{1}{2} \int e^{2x} dx = x \cdot \frac{1}{2} e^{2x} - \frac{1}{2} \cdot \frac{1}{2} e^{2x} + c$$

$$\int e^{2x} dx = \frac{1}{2} \int e^{2x} d2x = \frac{1}{2} e^{2x}$$

$$\int \underbrace{x}_u \cdot \underbrace{\cos x}_{dv} dx = \left| \begin{array}{l} u=x \quad du=dx \\ \cos x dx = dv \quad v = \sin x \end{array} \right| = x \cdot \sin x - \int \sin x dx = x \cdot \sin x + \cos x + c$$

$$1229. \int e^x \cos x \, dx. = \left| \begin{array}{l} u = \cos x \quad du = -\sin x \, dx \\ e^x \cdot dx = dv \quad v = e^x \end{array} \right| -$$

$$= \cos x \cdot e^x + \int e^x \cdot \sin x \, dx = \left| \begin{array}{l} u = \sin x \quad du = \cos x \, dx \\ e^x \cdot dx = dv \quad v = e^x \end{array} \right|$$

$$1229. \int e^x \cos x \, dx. = \cos x \cdot e^x + \sin x \cdot e^x - \int e^x \cdot \cos x \, dx$$

$$2 \int e^x \cdot \cos x \, dx = \cos x \cdot e^x + \sin x \cdot e^x$$

$$\int e^x \cdot \cos x \, dx = \frac{\cos x \cdot e^x + \sin x \cdot e^x}{2} + C$$

$$\int \underbrace{\arccos x}_u \, dx = \underbrace{\arccos x = u}_{dx = d} \quad \begin{array}{l} du = d \arccos x = -\frac{1}{\sqrt{1-x^2}} \, dx \\ v = x \end{array}$$

$$= x \cdot \arccos x + \int \underbrace{x}_{\text{circled}} \cdot \frac{1}{\sqrt{1-x^2}} \, dx = x \cdot \arccos x + \frac{1}{2} \int \frac{dx^2}{\sqrt{1-x^2}}$$

$$= x \cdot \arccos x - \frac{1}{2} \int (1-x^2)^{-\frac{1}{2}} d(1-x^2) -$$

$$= x \cdot \arccos x - \frac{1}{2} \cdot \frac{(1-x^2)^{-\frac{1}{2}+1}}{-\frac{1}{2}+1} + C$$

$$\int \frac{8m}{\sqrt{\ln x + 5}} \, dx$$

$$\int \frac{1 dx}{(x^2+16)^2} = \frac{1}{16} \int \frac{16 \cdot dx}{(x^2+16)^2} = \frac{1}{16} \int \frac{((x^2+16) - x^2) dx}{(x^2+16)^2} = \frac{1}{16} \int \left( \frac{1}{x^2+16} - \frac{x^2}{(x^2+16)^2} \right) dx$$

$$= \frac{1}{16} \left[ \int \frac{dx}{x^2+16} - \int \frac{x^2 dx}{(x^2+16)^2} \right]$$

$$\int \frac{x^2 dx}{(x^2+16)^2} = \int \frac{x \cdot x dx}{(x^2+16)^2} \quad \left| \begin{array}{l} u = x \\ dv = \frac{x \cdot dx}{(x^2+16)^2} \\ du = dx \\ v = -\frac{1}{2} \frac{1}{x^2+16} \end{array} \right. = -\frac{1}{2} \int \frac{1}{x^2+16}$$

$$\int \frac{x dx}{(x^2+16)^2} - \frac{1}{2} \int \frac{d(x^2+16)}{(x^2+16)^2} = \frac{1}{2} \int (x^2+16)^{-2} d(x^2+16) = -\frac{1}{2} \frac{1}{x^2+16}$$

$$= x \cdot \left( -\frac{1}{2} \cdot \frac{1}{x^2+16} \right) + \frac{1}{2} \int \frac{1}{x^2+16} dx$$

1216.  $\int \operatorname{arctg} x dx.$

1222.  $\int x^n \ln x dx.$

1232.  $\int \sqrt{1-x^2} dx.$

1235.  $\int e^{\operatorname{arcsin} x} dx.$

1233.  $\int \cos(\ln x) dx.$

$\int \operatorname{arctg} x dx = \left| u = \operatorname{arctg} x \quad du = (\operatorname{arctg} x)' \cdot dx = \frac{1}{1+x^2} dx \right| -$

$$\int \frac{1}{x} dx = \ln x \quad v = x$$

$$= x \cdot \arctan x - \int \frac{x dx}{1+x^2} = x \cdot \arctan x - \frac{1}{2} \int \frac{d(x^2+1)}{1+x^2} = x \cdot \arctan x - \frac{1}{2} \ln(x^2+1) + C$$

$$\int x^3 \cdot \ln x dx = \left| \begin{array}{l} u = \ln x \quad du = d \ln x = \frac{1}{x} dx \\ dv = x^3 dx \quad dv = d \frac{x^4}{4} \quad v = \frac{1}{4} x^4 \end{array} \right| = \ln x \cdot \frac{1}{4} x^4 - \frac{1}{4} \int x^4 \cdot \frac{1}{x} dx = \frac{1}{4} x^4 \ln x - \frac{1}{4} \int x^3 dx = \frac{1}{4} x^4 \ln x - \frac{1}{4} \frac{x^4}{4} + C$$

1232.  $\int \sqrt{1-x^2} dx$ . \*1235.  $\int e^{\arcsin x} dx$ .

1233.  $\int \cos(\ln x) dx$ .

$$\int \cos(\ln x) dx = \left| \begin{array}{l} u = \cos(\ln x) \quad du = d \cos(\ln x) = -\sin(\ln x) \cdot \frac{1}{x} dx \\ dv = dx \quad v = x \end{array} \right|$$

$$= \cos(\ln x) x - \int x \sin(\ln x) \cdot \frac{1}{x} dx = \left| \begin{array}{l} u = \sin(\ln x) \quad du = \cos(\ln x) \cdot \frac{1}{x} dx \\ dv = dx \quad v = x \end{array} \right|$$

$$= \cos(\ln x) \cdot x + \sin(\ln x) \cdot x - \int x \cos(\ln x) \cdot \frac{1}{x} dx$$

$$2 \int \cos(\ln x) dx = \cos(\ln x) \cdot x + \sin(\ln x) \cdot x$$

$$\int \cos(\ln x) dx = \frac{(\cos(\ln x) + \sin(\ln x)) \cdot x}{2} + C$$

$$\int \frac{(Ax+B)dx}{ax^2+bx+c}$$

$$\frac{P_n(x)}{Q_m(x)}$$

$$n < m$$

$$n \geq m$$

большее или равно  
и а

$$1254. \int \frac{5x^3 + 9x^2 - 22x - 8}{x^3 - 4x} dx.$$

$$\begin{array}{r} 5x^3 + 9x^2 - 22x - 8 \quad | \quad x^3 - 4x \\ - 5x^3 - 20x \\ \hline 9x^2 - 2x - 8 \end{array}$$

$$\frac{5}{3} \bigg| \frac{3}{2} \quad \frac{5}{3} = 1 + \frac{2}{3}$$

$$\frac{5x^3 + 9x^2 - 22x - 8}{x^3 - 4x} = 5 + \frac{9x^2 - 2x - 8}{x^3 - 4x}$$

$$\frac{P_n(x)}{Q_m(x)} = \frac{P_n(x)}{(x-a)^{\alpha} (x-b)^{\beta} \dots (x^2+cx+d)^{\gamma} \dots} = \frac{A}{x-a} + \frac{1}{(x-a)^2} + \dots + \frac{C}{(x-a)^{\alpha}} + \frac{D}{x-b} + \frac{E}{(x-b)^{\beta}} + \dots$$

$\alpha + \beta + \dots + \gamma + \dots$

$$+ \frac{F}{(x-b)^{\beta}} + \dots - \frac{Mx+K}{x^2+cx+d} + \frac{Lx+G}{(x^2+cx+d)^2} + \dots + \frac{Hx+I}{(x^2+cx+d)^{\gamma}} + \dots$$

$$2x - 4x - 8 \quad 0 \dots 2 \dots 0$$

$$\frac{5x^2 + 9x - 22x - 8}{x^3 - 4x} = 5 + \frac{5x - 22x - 8}{x^3 - 4x}$$

$$\boxed{\frac{9x^2 - 2x - 8}{x^3 - 4x} = \frac{9x^2 - 2x - 8}{x \cdot (x^2 - 4)} = \frac{9x^2 - 2x - 8}{x \cdot (x-2)(x+2)} = \frac{A}{x} + \frac{B}{x-2} + \frac{C}{x+2}}$$

$$= \frac{A \cdot \overbrace{(x-2)(x+2)}^{(x-2)(x+2)} + B \cdot \overbrace{x(x+2)}^{x(x+2)} + C \cdot \overbrace{x(x-2)}^{x(x-2)}}{x \cdot (x-2)(x+2)}$$

$$9x^2 - 2x - 8 = A \cdot (x-2)(x+2) + B \cdot x \cdot (x+2) + C \cdot x \cdot (x-2)$$

$$9x^2 - 2x - 8 = Ax^2 - 4A + Bx^2 + \underline{2Bx} + Cx^2 - \underline{2Cx}$$

$$9x^2 - 2x - 8 = x^2(A+B+C) + x \cdot (2B - 2C) + (-4A)$$

$$\begin{matrix} x^2 \\ x \\ x^0 \end{matrix} \begin{cases} 9 = A+B+C \\ -2 = 2B-2C \\ -8 = -4A \end{cases}$$

$$9x^2 - 2x - 8 = A \cdot (x-2)(x+2) + B \cdot x \cdot (x+2) + C \cdot x \cdot (x-2)$$

$$\underline{x=0} \quad -8 = A \cdot (-4) \Rightarrow A = 2$$

$$\underline{x=2} \quad 9 \cdot 4 - 2 \cdot 2 - 8 = B \cdot 2 \cdot 4 \Rightarrow B = 3$$

$$\underline{x=-2} \quad 9 \cdot 4 + 2 \cdot 2 - 8 = C \cdot (-2) \cdot (-4) \Rightarrow C = 4$$

$$\boxed{\frac{3x^2 - 2x - 8}{x^3 - 4x}} = \frac{A}{x} + \frac{B}{x-2} + \frac{C}{x+2} = \boxed{\frac{2}{x} + \frac{3}{x-2} + \frac{4}{x+2}}$$

$$I = \int \left( 5 + \frac{2}{x} + \frac{3}{x-2} + \frac{4}{x+2} \right) dx = 5x + 2 \ln|x| + 3 \ln|x-2| + 4 \ln|x+2| + C$$

$$1255. \int \frac{x^2 + x - 1}{x^3 + x^2 - 6x} dx = \frac{1}{6} \int \frac{dx}{x} + \frac{1}{2} \int \frac{dx}{x-2} + \frac{1}{3} \int \frac{dx}{x+3} = \frac{1}{6} \ln|x| + \frac{1}{2} \ln|x-2| + \frac{1}{3} \ln|x+3| + C$$

$$\frac{x^2 + x - 1}{x^3 + x^2 - 6x} = \frac{x^2 + x - 1}{x(x^2 + x - 6)} = \frac{x^2 + x - 1}{x(x-2)(x+3)} = \frac{A}{x} + \frac{B}{x-2} + \frac{C}{x+3} -$$

$$= \frac{A(x-2)(x+3) + B \cdot x \cdot (x+3) + C \cdot x(x-2)}{x \cdot (x-2)(x+3)}$$

$$\boxed{x^2 + x - 1 = A(x-2)(x+3) + B \cdot x \cdot (x+3) + C \cdot x \cdot (x-2)} \quad |$$

$$x=0 \quad -1 = -6A \quad A = \frac{1}{6}$$

$$x=2 \quad 5 = 10B \quad B = \frac{1}{2}$$

$$x=-3 \quad 5 = 15C \quad C = \frac{1}{3}$$

